<?xml version="1.0"?>
<rdf:RDF xmlns="https://www.theworldavatar.com/kg/ontobatchexperiment/"
     xml:base="https://www.theworldavatar.com/kg/ontobatchexperiment/"
     xmlns:dc="http://purl.org/dc/elements/1.1/"
     xmlns:owl="http://www.w3.org/2002/07/owl#"
     xmlns:rdf="http://www.w3.org/1999/02/22-rdf-syntax-ns#"
     xmlns:xml="http://www.w3.org/XML/1998/namespace"
     xmlns:xsd="http://www.w3.org/2001/XMLSchema#"
     xmlns:rdfs="http://www.w3.org/2000/01/rdf-schema#"
     xmlns:ontobatchexperiment="https://www.theworldavatar.com/kg/ontobatchexperiment/">
    <owl:Ontology rdf:about="https://www.theworldavatar.com/kg/ontobatchexperiment/">
        <dc:date>08 August 2024</dc:date>
        <rdfs:comment>OntoBatchExperiment is an ontology to represent batch experiments and relevant information.</rdfs:comment>
        <owl:versionInfo>1</owl:versionInfo>
        <gitCommitHash>c0599beca8df55873a1ab061dee64e52c510c6a0</gitCommitHash>
    </owl:Ontology>
    


    <!-- 
    ///////////////////////////////////////////////////////////////////////////////////////
    //
    // Annotation properties
    //
    ///////////////////////////////////////////////////////////////////////////////////////
     -->


    


    <!-- http://purl.org/dc/elements/1.1/date -->


    <owl:AnnotationProperty rdf:about="http://purl.org/dc/elements/1.1/date"/>
    


    <!-- https://www.theworldavatar.com/kg/ontobatchexperiment/gitCommitHash -->


    <owl:AnnotationProperty rdf:about="https://www.theworldavatar.com/kg/ontobatchexperiment/gitCommitHash"/>
    


    <!-- 
    ///////////////////////////////////////////////////////////////////////////////////////
    //
    // Object Properties
    //
    ///////////////////////////////////////////////////////////////////////////////////////
     -->


    


    <!-- https://www.theworldavatar.com/kg/ontobatchexperiment/hasAmountOfSubstanceConcentration -->


    <owl:ObjectProperty rdf:about="https://www.theworldavatar.com/kg/ontobatchexperiment/hasAmountOfSubstanceConcentration">
        <rdfs:domain rdf:resource="http://www.theworldavatar.com/ontology/ontocape/material/phase_system/phase_system.owl#PhaseComponent"/>
        <rdfs:range rdf:resource="http://www.ontology-of-units-of-measure.org/resource/om-2/AmountOfSubstanceConcentration"/>
        <rdfs:comment>A relationship between a phase component and its amount of substance concentration.</rdfs:comment>
        <rdfs:isDefinedBy rdf:resource="https://www.theworldavatar.com/kg/ontobatchexperiment/"/>
        <rdfs:label>has amount of substance concentration</rdfs:label>
    </owl:ObjectProperty>
    


    <!-- https://www.theworldavatar.com/kg/ontobatchexperiment/hasBatchExperimentCategory -->


    <owl:ObjectProperty rdf:about="https://www.theworldavatar.com/kg/ontobatchexperiment/hasBatchExperimentCategory">
        <rdfs:domain rdf:resource="https://www.theworldavatar.com/kg/ontobatchexperiment/BatchExperiment"/>
        <rdfs:range rdf:resource="https://www.theworldavatar.com/kg/ontobatchexperiment/BatchExperimentCategory"/>
        <rdfs:comment>A relationship to describe the category of a batch experiment.</rdfs:comment>
        <rdfs:isDefinedBy rdf:resource="https://www.theworldavatar.com/kg/ontobatchexperiment/"/>
        <rdfs:label>has batch experiment category</rdfs:label>
    </owl:ObjectProperty>
    


    <!-- https://www.theworldavatar.com/kg/ontobatchexperiment/hasBatchNumber -->


    <owl:ObjectProperty rdf:about="https://www.theworldavatar.com/kg/ontobatchexperiment/hasBatchNumber">
        <rdfs:domain rdf:resource="https://www.theworldavatar.com/kg/ontobatchexperiment/BatchExperiment"/>
        <rdfs:range rdf:resource="https://www.theworldavatar.com/kg/ontobatchexperiment/BatchNumber"/>
        <rdfs:comment>A relationship that describes the batch number allocated to a batch experiment.</rdfs:comment>
        <rdfs:isDefinedBy rdf:resource="https://www.theworldavatar.com/kg/ontobatchexperiment/"/>
        <rdfs:label>has batch number</rdfs:label>
    </owl:ObjectProperty>
    


    <!-- https://www.theworldavatar.com/kg/ontobatchexperiment/hasExpectedpHLevel -->


    <owl:ObjectProperty rdf:about="https://www.theworldavatar.com/kg/ontobatchexperiment/hasExpectedpHLevel">
        <rdfs:domain rdf:resource="http://www.theworldavatar.com/ontology/ontocape/material/phase_system/phase_system.owl#PhaseComponent"/>
        <rdfs:range rdf:resource="http://www.ontology-of-units-of-measure.org/resource/om-2/pHLevel"/>
        <rdfs:comment>A relationship between a phase component and its expected pH level.</rdfs:comment>
        <rdfs:isDefinedBy rdf:resource="https://www.theworldavatar.com/kg/ontobatchexperiment/"/>
        <rdfs:label>has expected pH level</rdfs:label>
    </owl:ObjectProperty>
    


    <!-- https://www.theworldavatar.com/kg/ontobatchexperiment/hasIdentifier -->


    <owl:ObjectProperty rdf:about="https://www.theworldavatar.com/kg/ontobatchexperiment/hasIdentifier">
        <rdfs:domain rdf:resource="https://www.theworldavatar.com/kg/ontobatchexperiment/BatchExperiment"/>
        <rdfs:range rdf:resource="https://www.theworldavatar.com/kg/ontobatchexperiment/Identifier"/>
        <rdfs:comment>A relationship that describes the identifier allocated to a batch experiment.</rdfs:comment>
        <rdfs:isDefinedBy rdf:resource="https://www.theworldavatar.com/kg/ontobatchexperiment/"/>
        <rdfs:label>has identifier</rdfs:label>
    </owl:ObjectProperty>
    


    <!-- https://www.theworldavatar.com/kg/ontobatchexperiment/hasMassFraction -->


    <owl:ObjectProperty rdf:about="https://www.theworldavatar.com/kg/ontobatchexperiment/hasMassFraction">
        <rdfs:domain rdf:resource="http://www.theworldavatar.com/ontology/ontocape/material/phase_system/phase_system.owl#PhaseComponent"/>
        <rdfs:range rdf:resource="http://www.ontology-of-units-of-measure.org/resource/om-2/MassFraction"/>
        <rdfs:comment>A relationship between a phase component and its mass fraction.</rdfs:comment>
        <rdfs:isDefinedBy rdf:resource="https://www.theworldavatar.com/kg/ontobatchexperiment/"/>
        <rdfs:label>has mass fraction</rdfs:label>
    </owl:ObjectProperty>
    


    <!-- https://www.theworldavatar.com/kg/ontobatchexperiment/hasWorkCode -->


    <owl:ObjectProperty rdf:about="https://www.theworldavatar.com/kg/ontobatchexperiment/hasWorkCode">
        <rdfs:domain rdf:resource="https://www.theworldavatar.com/kg/ontobatchexperiment/BatchExperiment"/>
        <rdfs:range rdf:resource="https://www.theworldavatar.com/kg/ontobatchexperiment/WorkCode"/>
        <rdfs:comment>A relationship that describes the work code allocated to a batch experiment.</rdfs:comment>
        <rdfs:isDefinedBy rdf:resource="https://www.theworldavatar.com/kg/ontobatchexperiment/"/>
        <rdfs:label>has work code</rdfs:label>
    </owl:ObjectProperty>
    


    <!-- https://www.theworldavatar.com/kg/ontobatchexperiment/haspHLevel -->


    <owl:ObjectProperty rdf:about="https://www.theworldavatar.com/kg/ontobatchexperiment/haspHLevel">
        <rdfs:domain rdf:resource="http://www.theworldavatar.com/ontology/ontocape/material/phase_system/phase_system.owl#PhaseComponent"/>
        <rdfs:range rdf:resource="http://www.ontology-of-units-of-measure.org/resource/om-2/pHLevel"/>
        <rdfs:comment>A relationship between a phase component and its pH level.</rdfs:comment>
        <rdfs:isDefinedBy rdf:resource="https://www.theworldavatar.com/kg/ontobatchexperiment/"/>
        <rdfs:label>has pH level</rdfs:label>
    </owl:ObjectProperty>
    


    <!-- https://www.theworldavatar.com/kg/ontoderivation/belongsTo -->


    <owl:ObjectProperty rdf:about="https://www.theworldavatar.com/kg/ontoderivation/belongsTo">
        <rdfs:domain rdf:resource="https://www.theworldavatar.com/kg/ontobatchexperiment/Identifier"/>
        <rdfs:range rdf:resource="https://www.theworldavatar.com/kg/ontoderivation/Derivation"/>
        <rdfs:isDefinedBy rdf:resource="https://www.theworldavatar.com/kg/ontobatchexperiment/"/>
        <rdfs:label>belongs to</rdfs:label>
    </owl:ObjectProperty>
    


    <!-- https://www.theworldavatar.com/kg/ontoderivation/isDerivedFrom -->


    <owl:ObjectProperty rdf:about="https://www.theworldavatar.com/kg/ontoderivation/isDerivedFrom">
        <rdfs:domain rdf:resource="https://www.theworldavatar.com/kg/ontoderivation/Derivation"/>
        <rdfs:range>
            <owl:Class>
                <owl:unionOf rdf:parseType="Collection">
                    <rdf:Description rdf:about="https://www.theworldavatar.com/kg/ontobatchexperiment/BatchExperimentCategory"/>
                    <rdf:Description rdf:about="https://www.theworldavatar.com/kg/ontobatchexperiment/BatchNumber"/>
                    <rdf:Description rdf:about="https://www.theworldavatar.com/kg/ontobatchexperiment/WorkCode"/>
                    <rdf:Description rdf:about="https://www.theworldavatar.com/kg/ontoprofile/Initials"/>
                </owl:unionOf>
            </owl:Class>
        </rdfs:range>
        <rdfs:comment>A relationship to describe an identifier being derived from other types of information.</rdfs:comment>
        <rdfs:isDefinedBy rdf:resource="https://www.theworldavatar.com/kg/ontobatchexperiment/"/>
        <rdfs:label>is derived from</rdfs:label>
    </owl:ObjectProperty>
    


    <!-- 
    ///////////////////////////////////////////////////////////////////////////////////////
    //
    // Classes
    //
    ///////////////////////////////////////////////////////////////////////////////////////
     -->


    


    <!-- http://www.ontology-of-units-of-measure.org/resource/om-2/AmountOfSubstanceConcentration -->


    <owl:Class rdf:about="http://www.ontology-of-units-of-measure.org/resource/om-2/AmountOfSubstanceConcentration"/>
    


    <!-- http://www.ontology-of-units-of-measure.org/resource/om-2/MassFraction -->


    <owl:Class rdf:about="http://www.ontology-of-units-of-measure.org/resource/om-2/MassFraction"/>
    


    <!-- http://www.ontology-of-units-of-measure.org/resource/om-2/pHLevel -->


    <owl:Class rdf:about="http://www.ontology-of-units-of-measure.org/resource/om-2/pHLevel"/>
    


    <!-- http://www.theworldavatar.com/ontology/ontocape/material/phase_system/phase_system.owl#PhaseComponent -->


    <owl:Class rdf:about="http://www.theworldavatar.com/ontology/ontocape/material/phase_system/phase_system.owl#PhaseComponent"/>
    


    <!-- https://www.theworldavatar.com/kg/ontobatchexperiment/BatchExperiment -->


    <owl:Class rdf:about="https://www.theworldavatar.com/kg/ontobatchexperiment/BatchExperiment">
        <rdfs:subClassOf rdf:resource="https://www.theworldavatar.com/kg/ontoreaction/ReactionExperiment"/>
        <rdfs:comment>A type of experiment or process in which a fixed quantity of materials is processed together in a single batch or lot.</rdfs:comment>
        <rdfs:isDefinedBy rdf:resource="https://www.theworldavatar.com/kg/ontobatchexperiment/"/>
        <rdfs:label>Batch experiment</rdfs:label>
    </owl:Class>
    


    <!-- https://www.theworldavatar.com/kg/ontobatchexperiment/BatchExperimentCategory -->


    <owl:Class rdf:about="https://www.theworldavatar.com/kg/ontobatchexperiment/BatchExperimentCategory">
        <rdfs:comment>A classification or type of batch experiment based on specific criteria or characteristics.</rdfs:comment>
        <rdfs:isDefinedBy rdf:resource="https://www.theworldavatar.com/kg/ontobatchexperiment/"/>
        <rdfs:label>Batch experiment category</rdfs:label>
    </owl:Class>
    


    <!-- https://www.theworldavatar.com/kg/ontobatchexperiment/BatchNumber -->


    <owl:Class rdf:about="https://www.theworldavatar.com/kg/ontobatchexperiment/BatchNumber">
        <rdfs:comment>A number assigned to a batch experiment.</rdfs:comment>
        <rdfs:isDefinedBy rdf:resource="https://www.theworldavatar.com/kg/ontobatchexperiment/"/>
        <rdfs:label>Batch number</rdfs:label>
    </owl:Class>
    


    <!-- https://www.theworldavatar.com/kg/ontobatchexperiment/Identifier -->


    <owl:Class rdf:about="https://www.theworldavatar.com/kg/ontobatchexperiment/Identifier">
        <rdfs:comment>A unique identifier assigned to a batch experiment that is derived from other types of information (e.g. work code, batch number, initials, BatchExperimentCategory).</rdfs:comment>
        <rdfs:isDefinedBy rdf:resource="https://www.theworldavatar.com/kg/ontobatchexperiment/"/>
        <rdfs:label>Identifier</rdfs:label>
    </owl:Class>
    


    <!-- https://www.theworldavatar.com/kg/ontobatchexperiment/WorkCode -->


    <owl:Class rdf:about="https://www.theworldavatar.com/kg/ontobatchexperiment/WorkCode">
        <rdfs:comment>A confidential internal identifier assigned to a batch experiment.</rdfs:comment>
        <rdfs:isDefinedBy rdf:resource="https://www.theworldavatar.com/kg/ontobatchexperiment/"/>
        <rdfs:label>Work code</rdfs:label>
    </owl:Class>
    


    <!-- https://www.theworldavatar.com/kg/ontoderivation/Derivation -->


    <owl:Class rdf:about="https://www.theworldavatar.com/kg/ontoderivation/Derivation">
        <rdfs:comment>Synchronous derivation</rdfs:comment>
        <rdfs:isDefinedBy rdf:resource="https://www.theworldavatar.com/kg/ontoderivation/"/>
        <rdfs:label>Derivation</rdfs:label>
    </owl:Class>
    


    <!-- https://www.theworldavatar.com/kg/ontoprofile/Initials -->


    <owl:Class rdf:about="https://www.theworldavatar.com/kg/ontoprofile/Initials"/>
    


    <!-- https://www.theworldavatar.com/kg/ontoreaction/ReactionExperiment -->


    <owl:Class rdf:about="https://www.theworldavatar.com/kg/ontoreaction/ReactionExperiment"/>
</rdf:RDF>



<!-- Generated by the OWL API (version 5.5.0.2023-01-14T12:41:38Z) https://github.com/owlcs/owlapi/ -->


