<?xml version="1.0"?>
<rdf:RDF xmlns="https://theworldavatar.io/kg/ontochangelog/"
     xml:base="https://theworldavatar.io/kg/ontochangelog/"
     xmlns:dc="http://purl.org/dc/elements/1.1/"
     xmlns:owl="http://www.w3.org/2002/07/owl#"
     xmlns:rdf="http://www.w3.org/1999/02/22-rdf-syntax-ns#"
     xmlns:xml="http://www.w3.org/XML/1998/namespace"
     xmlns:xsd="http://www.w3.org/2001/XMLSchema#"
     xmlns:rdfs="http://www.w3.org/2000/01/rdf-schema#"
     xmlns:ontochangelog="https://theworldavatar.io/kg/ontochangelog/">
    <owl:Ontology rdf:about="https://theworldavatar.io/kg/ontochangelog/">
        <dc:date>20 January 2026</dc:date>
        <rdfs:comment>The OntoChangelog ontology provides a clear history of every change, acting as a digital paper trail that records who made a change, when it occurred, and a description of the action.</rdfs:comment>
        <owl:versionInfo>1</owl:versionInfo>
        <gitCommitHash>c0599beca8df55873a1ab061dee64e52c510c6a0</gitCommitHash>
    </owl:Ontology>
    


    <!-- 
    ///////////////////////////////////////////////////////////////////////////////////////
    //
    // Annotation properties
    //
    ///////////////////////////////////////////////////////////////////////////////////////
     -->


    


    <!-- http://purl.org/dc/elements/1.1/date -->


    <owl:AnnotationProperty rdf:about="http://purl.org/dc/elements/1.1/date"/>
    


    <!-- https://theworldavatar.io/kg/ontochangelog/gitCommitHash -->


    <owl:AnnotationProperty rdf:about="https://theworldavatar.io/kg/ontochangelog/gitCommitHash"/>
    


    <!-- 
    ///////////////////////////////////////////////////////////////////////////////////////
    //
    // Object Properties
    //
    ///////////////////////////////////////////////////////////////////////////////////////
     -->


    


    <!-- https://theworldavatar.io/kg/ontochangelog/affected -->


    <owl:ObjectProperty rdf:about="https://theworldavatar.io/kg/ontochangelog/affected">
        <rdfs:domain rdf:resource="https://theworldavatar.io/kg/ontochangelog/Activity"/>
        <rdfs:comment>A relationship that defines the specific object, record, or piece of data that was changed during the activity.</rdfs:comment>
        <rdfs:isDefinedBy rdf:resource="https://theworldavatar.io/kg/ontochangelog/"/>
        <rdfs:label>affected</rdfs:label>
    </owl:ObjectProperty>
    


    <!-- https://theworldavatar.io/kg/ontochangelog/wasPerformedBy -->


    <owl:ObjectProperty rdf:about="https://theworldavatar.io/kg/ontochangelog/wasPerformedBy">
        <rdfs:domain rdf:resource="https://theworldavatar.io/kg/ontochangelog/Activity"/>
        <rdfs:range rdf:resource="http://xmlns.com/foaf/0.1/Agent"/>
        <rdfs:comment>A relationship that defines the individual or automated system responsible for triggering the activity.</rdfs:comment>
        <rdfs:isDefinedBy rdf:resource="https://theworldavatar.io/kg/ontochangelog/"/>
        <rdfs:label>was performed by</rdfs:label>
    </owl:ObjectProperty>
    


    <!-- 
    ///////////////////////////////////////////////////////////////////////////////////////
    //
    // Data properties
    //
    ///////////////////////////////////////////////////////////////////////////////////////
     -->


    


    <!-- https://theworldavatar.io/kg/ontochangelog/timestamp -->


    <owl:DatatypeProperty rdf:about="https://theworldavatar.io/kg/ontochangelog/timestamp">
        <rdfs:domain rdf:resource="https://theworldavatar.io/kg/ontochangelog/Activity"/>
        <rdfs:range rdf:resource="http://www.w3.org/2001/XMLSchema#string"/>
        <rdfs:comment>A property to store the precise date and time when the activity was completed.</rdfs:comment>
        <rdfs:isDefinedBy rdf:resource="https://theworldavatar.io/kg/ontochangelog/"/>
        <rdfs:label>timestamp</rdfs:label>
    </owl:DatatypeProperty>
    


    <!-- 
    ///////////////////////////////////////////////////////////////////////////////////////
    //
    // Classes
    //
    ///////////////////////////////////////////////////////////////////////////////////////
     -->


    


    <!-- http://xmlns.com/foaf/0.1/Agent -->


    <owl:Class rdf:about="http://xmlns.com/foaf/0.1/Agent"/>
    


    <!-- https://theworldavatar.io/kg/ontochangelog/Activity -->


    <owl:Class rdf:about="https://theworldavatar.io/kg/ontochangelog/Activity">
        <rdfs:comment>A specific event or process where a change occurs.</rdfs:comment>
        <rdfs:isDefinedBy rdf:resource="https://theworldavatar.io/kg/ontochangelog/"/>
        <rdfs:label>Activity</rdfs:label>
    </owl:Class>
</rdf:RDF>



<!-- Generated by the OWL API (version 5.5.0.2023-01-14T12:41:38Z) https://github.com/owlcs/owlapi/ -->


