<?xml version="1.0"?>
<rdf:RDF xmlns="https://github.com/TheWorldAvatar/ontoclimateadapt#"
     xml:base="https://github.com/TheWorldAvatar/ontoclimateadapt"
     xmlns:dc="http://purl.org/dc/elements/1.1/"
     xmlns:owl="http://www.w3.org/2002/07/owl#"
     xmlns:rdf="http://www.w3.org/1999/02/22-rdf-syntax-ns#"
     xmlns:xml="http://www.w3.org/XML/1998/namespace"
     xmlns:xsd="http://www.w3.org/2001/XMLSchema#"
     xmlns:rdfs="http://www.w3.org/2000/01/rdf-schema#"
     xmlns:ontoclimateadapt="https://github.com/TheWorldAvatar/ontoclimateadapt#">
    <owl:Ontology rdf:about="https://github.com/TheWorldAvatar/ontoclimateadapt">
        <dc:date>26 January 2026</dc:date>
        <rdfs:comment>OntoClimateAdapt is an ontology designed to provide a formal semantic representation of data related to climate change adaptation research, initiatives, and actions. It enables the standardized description, integration, and interoperable exchange of information to support the development of resilient societies and adaptive capacities in the face of climate change.</rdfs:comment>
        <owl:versionInfo>1</owl:versionInfo>
        <gitCommitHash>c0599beca8df55873a1ab061dee64e52c510c6a0</gitCommitHash>
    </owl:Ontology>
    


    <!-- 
    ///////////////////////////////////////////////////////////////////////////////////////
    //
    // Annotation properties
    //
    ///////////////////////////////////////////////////////////////////////////////////////
     -->


    


    <!-- http://purl.org/dc/elements/1.1/date -->


    <owl:AnnotationProperty rdf:about="http://purl.org/dc/elements/1.1/date"/>
    


    <!-- https://github.com/TheWorldAvatar/ontoclimateadapt#gitCommitHash -->


    <owl:AnnotationProperty rdf:about="https://github.com/TheWorldAvatar/ontoclimateadapt#gitCommitHash"/>
    


    <!-- 
    ///////////////////////////////////////////////////////////////////////////////////////
    //
    // Object Properties
    //
    ///////////////////////////////////////////////////////////////////////////////////////
     -->


    


    <!-- http://www.ontology-of-units-of-measure.org/resource/om-2/hasUnit -->


    <owl:ObjectProperty rdf:about="http://www.ontology-of-units-of-measure.org/resource/om-2/hasUnit">
        <rdfs:domain rdf:resource="http://www.ontology-of-units-of-measure.org/resource/om-2/Measure"/>
        <rdfs:range rdf:resource="http://www.ontology-of-units-of-measure.org/resource/om-2/Unit"/>
        <rdfs:isDefinedBy rdf:resource="http://www.ontology-of-units-of-measure.org/resource/om-2/"/>
        <rdfs:label>hasUnit</rdfs:label>
    </owl:ObjectProperty>
    


    <!-- http://www.ontology-of-units-of-measure.org/resource/om-2/hasValue -->


    <owl:ObjectProperty rdf:about="http://www.ontology-of-units-of-measure.org/resource/om-2/hasValue">
        <rdfs:domain rdf:resource="http://www.ontology-of-units-of-measure.org/resource/om-2/Quantity"/>
        <rdfs:range rdf:resource="http://www.ontology-of-units-of-measure.org/resource/om-2/Measure"/>
        <rdfs:isDefinedBy rdf:resource="http://www.ontology-of-units-of-measure.org/resource/om-2/"/>
        <rdfs:label>hasValue</rdfs:label>
    </owl:ObjectProperty>
    


    <!-- http://www.w3.org/2006/time#hasBeginning -->


    <owl:ObjectProperty rdf:about="http://www.w3.org/2006/time#hasBeginning">
        <rdfs:domain rdf:resource="http://www.w3.org/2006/time#TemporalEntity"/>
        <rdfs:range rdf:resource="http://www.w3.org/2006/time#Instant"/>
        <rdfs:isDefinedBy rdf:resource="http://www.w3.org/2006/time"/>
        <rdfs:label>hasBeginning</rdfs:label>
    </owl:ObjectProperty>
    


    <!-- http://www.w3.org/2006/time#hasEnd -->


    <owl:ObjectProperty rdf:about="http://www.w3.org/2006/time#hasEnd">
        <rdfs:domain rdf:resource="http://www.w3.org/2006/time#TemporalEntity"/>
        <rdfs:range rdf:resource="http://www.w3.org/2006/time#Instant"/>
        <rdfs:isDefinedBy rdf:resource="http://www.w3.org/2006/time"/>
        <rdfs:label>hasEnd</rdfs:label>
    </owl:ObjectProperty>
    


    <!-- https://github.com/TheWorldAvatar/ontoclimateadapt#adaptedThrough -->


    <owl:ObjectProperty rdf:about="https://github.com/TheWorldAvatar/ontoclimateadapt#adaptedThrough">
        <rdfs:domain rdf:resource="https://github.com/TheWorldAvatar/ontoclimateadapt#ClimateChange"/>
        <rdfs:range rdf:resource="https://github.com/TheWorldAvatar/ontoclimateadapt#AdaptationMeasure"/>
        <rdfs:isDefinedBy rdf:resource="https://github.com/TheWorldAvatar/ontoclimateadapt"/>
        <rdfs:label>adaptedThrough</rdfs:label>
    </owl:ObjectProperty>
    


    <!-- https://github.com/TheWorldAvatar/ontoclimateadapt#affects -->


    <owl:ObjectProperty rdf:about="https://github.com/TheWorldAvatar/ontoclimateadapt#affects">
        <rdfs:domain rdf:resource="https://github.com/TheWorldAvatar/ontoclimateadapt#ClimateChange"/>
        <rdfs:range>
            <owl:Class>
                <owl:unionOf rdf:parseType="Collection">
                    <rdf:Description rdf:about="https://github.com/TheWorldAvatar/ontoclimateadapt#Ecology"/>
                    <rdf:Description rdf:about="https://github.com/TheWorldAvatar/ontoclimateadapt#Economy"/>
                    <rdf:Description rdf:about="https://github.com/TheWorldAvatar/ontoclimateadapt#HumanHealth"/>
                </owl:unionOf>
            </owl:Class>
        </rdfs:range>
        <rdfs:comment>An influence relationship between a phenomenon, process, or event and the systems, entities, or domains that experience its impact.</rdfs:comment>
        <rdfs:isDefinedBy rdf:resource="https://github.com/TheWorldAvatar/ontoclimateadapt"/>
        <rdfs:label>affects</rdfs:label>
    </owl:ObjectProperty>
    


    <!-- https://github.com/TheWorldAvatar/ontoclimateadapt#forAgeGroup -->


    <owl:ObjectProperty rdf:about="https://github.com/TheWorldAvatar/ontoclimateadapt#forAgeGroup">
        <rdfs:domain rdf:resource="https://github.com/TheWorldAvatar/ontoclimateadapt#AgeSpecificPopulationDensity"/>
        <rdfs:range rdf:resource="https://github.com/TheWorldAvatar/ontoclimateadapt#AgeGroup"/>
        <rdfs:comment>A relation indicating that a population density measurement applies to a specific age group defined by a minimum and maximum age.</rdfs:comment>
        <rdfs:isDefinedBy rdf:resource="https://github.com/TheWorldAvatar/ontoclimateadapt"/>
        <rdfs:label>forAgeGroup</rdfs:label>
    </owl:ObjectProperty>
    


    <!-- https://github.com/TheWorldAvatar/ontoclimateadapt#hasCause -->


    <owl:ObjectProperty rdf:about="https://github.com/TheWorldAvatar/ontoclimateadapt#hasCause">
        <rdfs:domain rdf:resource="https://github.com/TheWorldAvatar/ontoclimateadapt#ClimateChange"/>
        <rdfs:range rdf:resource="https://github.com/TheWorldAvatar/ontoclimateadapt#GreenhouseGasEmission"/>
        <rdfs:comment>A causal relationship between an effect (or phenomenon) and the process, or event responsible for its occurrence.</rdfs:comment>
        <rdfs:isDefinedBy rdf:resource="https://github.com/TheWorldAvatar/ontoclimateadapt"/>
        <rdfs:label>hasCause</rdfs:label>
    </owl:ObjectProperty>
    


    <!-- https://github.com/TheWorldAvatar/ontoclimateadapt#hasEffect -->


    <owl:ObjectProperty rdf:about="https://github.com/TheWorldAvatar/ontoclimateadapt#hasEffect">
        <rdfs:domain rdf:resource="https://github.com/TheWorldAvatar/ontoclimateadapt#ClimateChange"/>
        <rdfs:range>
            <owl:Class>
                <owl:unionOf rdf:parseType="Collection">
                    <rdf:Description rdf:about="https://github.com/TheWorldAvatar/ontoclimateadapt#MeteorologicalExtremeEvent"/>
                    <rdf:Description rdf:about="https://github.com/TheWorldAvatar/ontoclimateadapt#OceanAcidification"/>
                    <rdf:Description rdf:about="https://github.com/TheWorldAvatar/ontoclimateadapt#SeaLevelRise"/>
                </owl:unionOf>
            </owl:Class>
        </rdfs:range>
        <rdfs:comment>A causal relationship between a phenomenon and the observable processes, events, or conditions that result from it.</rdfs:comment>
        <rdfs:isDefinedBy rdf:resource="https://github.com/TheWorldAvatar/ontoclimateadapt"/>
        <rdfs:label>hasEffect</rdfs:label>
    </owl:ObjectProperty>
    


    <!-- https://github.com/TheWorldAvatar/ontoclimateadapt#hasFrequency -->


    <owl:ObjectProperty rdf:about="https://github.com/TheWorldAvatar/ontoclimateadapt#hasFrequency">
        <rdfs:domain rdf:resource="https://github.com/TheWorldAvatar/ontoclimateadapt#NumberOfHeatwaveDays"/>
        <rdfs:range rdf:resource="https://github.com/TheWorldAvatar/ontoclimateadapt#TemporalFrequency"/>
        <rdfs:comment>An object property that links an observation to the temporal frequency at which the observed quantity is defined, measured, or aggregated.</rdfs:comment>
        <rdfs:isDefinedBy rdf:resource="https://github.com/TheWorldAvatar/ontoclimateadapt"/>
        <rdfs:label>hasFrequency</rdfs:label>
    </owl:ObjectProperty>
    


    <!-- https://github.com/TheWorldAvatar/ontoclimateadapt#hasNumberOfHeatwaveDays -->


    <owl:ObjectProperty rdf:about="https://github.com/TheWorldAvatar/ontoclimateadapt#hasNumberOfHeatwaveDays">
        <rdfs:domain rdf:resource="https://github.com/TheWorldAvatar/ontoclimateadapt#Location"/>
        <rdfs:range rdf:resource="https://github.com/TheWorldAvatar/ontoclimateadapt#NumberOfHeatwaveDays"/>
        <rdfs:comment>An object property that relates a location to an observation representing the number of days during which heatwave conditions occur.</rdfs:comment>
        <rdfs:isDefinedBy rdf:resource="https://github.com/TheWorldAvatar/ontoclimateadapt"/>
        <rdfs:label>hasNumberOfHeatwaveDays</rdfs:label>
    </owl:ObjectProperty>
    


    <!-- https://github.com/TheWorldAvatar/ontoclimateadapt#hasPopulationDensity -->


    <owl:ObjectProperty rdf:about="https://github.com/TheWorldAvatar/ontoclimateadapt#hasPopulationDensity">
        <rdfs:domain rdf:resource="https://github.com/TheWorldAvatar/ontoclimateadapt#Location"/>
        <rdfs:range rdf:resource="https://github.com/TheWorldAvatar/ontoclimateadapt#PopulationDensity"/>
        <rdfs:comment>Relates a Location to its corresponding PopulationDensity measurement.</rdfs:comment>
        <rdfs:isDefinedBy rdf:resource="https://github.com/TheWorldAvatar/ontoclimateadapt"/>
        <rdfs:label>hasPopulationDensity</rdfs:label>
    </owl:ObjectProperty>
    


    <!-- https://github.com/TheWorldAvatar/ontoclimateadapt#hasTemperature -->


    <owl:ObjectProperty rdf:about="https://github.com/TheWorldAvatar/ontoclimateadapt#hasTemperature">
        <rdfs:domain rdf:resource="https://github.com/TheWorldAvatar/ontoclimateadapt#Location"/>
        <rdfs:range rdf:resource="http://www.ontology-of-units-of-measure.org/resource/om-2/Temperature"/>
        <rdfs:comment>An object property that relates a location to a temperature quantity describing the thermal state of that location at a specific time.</rdfs:comment>
        <rdfs:isDefinedBy rdf:resource="https://github.com/TheWorldAvatar/ontoclimateadapt"/>
        <rdfs:label>hasTemperature</rdfs:label>
    </owl:ObjectProperty>
    


    <!-- https://github.com/TheWorldAvatar/ontoclimateadapt#hasTimeInterval -->


    <owl:ObjectProperty rdf:about="https://github.com/TheWorldAvatar/ontoclimateadapt#hasTimeInterval">
        <rdfs:domain rdf:resource="https://github.com/TheWorldAvatar/ontoclimateadapt#NumberOfHeatwaveDays"/>
        <rdfs:range rdf:resource="http://www.w3.org/2006/time#TemporalEntity"/>
        <rdfs:comment>An object property that relates an aggregated observation result to the temporal interval over which it was computed.</rdfs:comment>
        <rdfs:isDefinedBy rdf:resource="https://github.com/TheWorldAvatar/ontoclimateadapt"/>
        <rdfs:label>hasTimeInterval</rdfs:label>
    </owl:ObjectProperty>
    


    <!-- https://github.com/TheWorldAvatar/ontoclimateadapt#isDerivedFromEvent -->


    <owl:ObjectProperty rdf:about="https://github.com/TheWorldAvatar/ontoclimateadapt#isDerivedFromEvent">
        <rdfs:domain rdf:resource="https://github.com/TheWorldAvatar/ontoclimateadapt#NumberOfHeatwaveDays"/>
        <rdfs:range rdf:resource="https://github.com/TheWorldAvatar/ontoclimateadapt#Heatwave"/>
        <rdfs:comment>An object property that relates a derived quantitative indicator to one or more events from which the indicator has been computed or aggregated.</rdfs:comment>
        <rdfs:isDefinedBy rdf:resource="https://github.com/TheWorldAvatar/ontoclimateadapt"/>
        <rdfs:label>isDerivedFromEvent</rdfs:label>
    </owl:ObjectProperty>
    


    <!-- https://github.com/TheWorldAvatar/ontoclimateadapt#measuredBy -->


    <owl:ObjectProperty rdf:about="https://github.com/TheWorldAvatar/ontoclimateadapt#measuredBy">
        <rdfs:domain rdf:resource="https://github.com/TheWorldAvatar/ontoclimateadapt#ClimateChange"/>
        <rdfs:range>
            <owl:Class>
                <owl:unionOf rdf:parseType="Collection">
                    <rdf:Description rdf:about="https://github.com/TheWorldAvatar/ontoclimateadapt#ClimateModel"/>
                    <rdf:Description rdf:about="https://github.com/TheWorldAvatar/ontoclimateadapt#MeteorologicalStation"/>
                    <rdf:Description rdf:about="https://github.com/TheWorldAvatar/ontoclimateadapt#SatelliteObservation"/>
                </owl:unionOf>
            </owl:Class>
        </rdfs:range>
        <rdfs:comment>The source of measurement, estimation, or observation through which evidence of climate change is obtained.</rdfs:comment>
        <rdfs:isDefinedBy rdf:resource="https://github.com/TheWorldAvatar/ontoclimateadapt"/>
        <rdfs:label>measuredBy</rdfs:label>
    </owl:ObjectProperty>
    


    <!-- https://github.com/TheWorldAvatar/ontoclimateadapt#occursAt -->


    <owl:ObjectProperty rdf:about="https://github.com/TheWorldAvatar/ontoclimateadapt#occursAt">
        <rdfs:domain rdf:resource="https://github.com/TheWorldAvatar/ontoclimateadapt#MeteorologicalExtremeEvent"/>
        <rdfs:range rdf:resource="https://github.com/TheWorldAvatar/ontoclimateadapt#Location"/>
        <rdfs:comment>A relation linking an event to the geographical location where it takes place or manifests its observable impacts.</rdfs:comment>
        <rdfs:isDefinedBy rdf:resource="https://github.com/TheWorldAvatar/ontoclimateadapt"/>
        <rdfs:label>occursAt</rdfs:label>
    </owl:ObjectProperty>
    


    <!-- https://github.com/TheWorldAvatar/ontoclimateadapt#studiedBy -->


    <owl:ObjectProperty rdf:about="https://github.com/TheWorldAvatar/ontoclimateadapt#studiedBy">
        <rdfs:domain rdf:resource="https://github.com/TheWorldAvatar/ontoclimateadapt#ClimateChange"/>
        <rdfs:range>
            <owl:Class>
                <owl:unionOf rdf:parseType="Collection">
                    <rdf:Description rdf:about="https://github.com/TheWorldAvatar/ontoclimateadapt#AtmosphericScience"/>
                    <rdf:Description rdf:about="https://github.com/TheWorldAvatar/ontoclimateadapt#EnvironmentalScience"/>
                    <rdf:Description rdf:about="https://github.com/TheWorldAvatar/ontoclimateadapt#Paleoclimatology"/>
                </owl:unionOf>
            </owl:Class>
        </rdfs:range>
        <rdfs:comment>The relationship between a natural or environmental phenomenon and the scientific disciplines that systematically investigate it.</rdfs:comment>
        <rdfs:isDefinedBy rdf:resource="https://github.com/TheWorldAvatar/ontoclimateadapt"/>
        <rdfs:label>studiedBy</rdfs:label>
    </owl:ObjectProperty>
    


    <!-- 
    ///////////////////////////////////////////////////////////////////////////////////////
    //
    // Data properties
    //
    ///////////////////////////////////////////////////////////////////////////////////////
     -->


    


    <!-- http://www.ontology-of-units-of-measure.org/resource/om-2/hasNumericalValue -->


    <owl:DatatypeProperty rdf:about="http://www.ontology-of-units-of-measure.org/resource/om-2/hasNumericalValue">
        <rdfs:domain rdf:resource="http://www.ontology-of-units-of-measure.org/resource/om-2/Measure"/>
        <rdfs:range rdf:resource="http://www.w3.org/2001/XMLSchema#double"/>
        <rdfs:isDefinedBy rdf:resource="http://www.ontology-of-units-of-measure.org/resource/om-2/"/>
        <rdfs:label>hasNumericalValue</rdfs:label>
    </owl:DatatypeProperty>
    


    <!-- http://www.ontology-of-units-of-measure.org/resource/om-2/symbol -->


    <owl:DatatypeProperty rdf:about="http://www.ontology-of-units-of-measure.org/resource/om-2/symbol">
        <rdfs:domain rdf:resource="http://www.ontology-of-units-of-measure.org/resource/om-2/Unit"/>
        <rdfs:range rdf:resource="http://www.w3.org/2001/XMLSchema#string"/>
        <rdfs:isDefinedBy rdf:resource="http://www.ontology-of-units-of-measure.org/resource/om-2/"/>
        <rdfs:label>symbol</rdfs:label>
    </owl:DatatypeProperty>
    


    <!-- http://www.w3.org/2006/time#inXSDDate -->


    <owl:DatatypeProperty rdf:about="http://www.w3.org/2006/time#inXSDDate">
        <rdfs:domain rdf:resource="http://www.w3.org/2006/time#Instant"/>
        <rdfs:range rdf:resource="http://www.w3.org/2001/XMLSchema#string"/>
        <rdfs:isDefinedBy rdf:resource="http://www.w3.org/2006/time"/>
        <rdfs:label>inXSDDate</rdfs:label>
    </owl:DatatypeProperty>
    


    <!-- https://github.com/TheWorldAvatar/ontoclimateadapt#hasMaximumAge -->


    <owl:DatatypeProperty rdf:about="https://github.com/TheWorldAvatar/ontoclimateadapt#hasMaximumAge">
        <rdfs:domain rdf:resource="https://github.com/TheWorldAvatar/ontoclimateadapt#AgeGroup"/>
        <rdfs:range rdf:resource="http://www.w3.org/2001/XMLSchema#integer"/>
        <rdfs:comment>A data property that specifies the upper bound of the age range defining an age group.</rdfs:comment>
        <rdfs:isDefinedBy rdf:resource="https://github.com/TheWorldAvatar/ontoclimateadapt"/>
        <rdfs:label>hasMaximumAge</rdfs:label>
    </owl:DatatypeProperty>
    


    <!-- https://github.com/TheWorldAvatar/ontoclimateadapt#hasMinimumAge -->


    <owl:DatatypeProperty rdf:about="https://github.com/TheWorldAvatar/ontoclimateadapt#hasMinimumAge">
        <rdfs:domain rdf:resource="https://github.com/TheWorldAvatar/ontoclimateadapt#AgeGroup"/>
        <rdfs:range rdf:resource="http://www.w3.org/2001/XMLSchema#integer"/>
        <rdfs:comment>A data property that specifies the lower bound of the age range defining an age group.</rdfs:comment>
        <rdfs:isDefinedBy rdf:resource="https://github.com/TheWorldAvatar/ontoclimateadapt"/>
        <rdfs:label>hasMinimumAge</rdfs:label>
    </owl:DatatypeProperty>
    


    <!-- 
    ///////////////////////////////////////////////////////////////////////////////////////
    //
    // Classes
    //
    ///////////////////////////////////////////////////////////////////////////////////////
     -->


    


    <!-- http://www.ontology-of-units-of-measure.org/resource/om-2/Measure -->


    <owl:Class rdf:about="http://www.ontology-of-units-of-measure.org/resource/om-2/Measure"/>
    


    <!-- http://www.ontology-of-units-of-measure.org/resource/om-2/Quantity -->


    <owl:Class rdf:about="http://www.ontology-of-units-of-measure.org/resource/om-2/Quantity"/>
    


    <!-- http://www.ontology-of-units-of-measure.org/resource/om-2/Temperature -->


    <owl:Class rdf:about="http://www.ontology-of-units-of-measure.org/resource/om-2/Temperature">
        <rdfs:subClassOf rdf:resource="http://www.ontology-of-units-of-measure.org/resource/om-2/Quantity"/>
        <rdfs:isDefinedBy rdf:resource="http://www.ontology-of-units-of-measure.org/resource/om-2/"/>
        <rdfs:label>Temperature</rdfs:label>
    </owl:Class>
    


    <!-- http://www.ontology-of-units-of-measure.org/resource/om-2/Unit -->


    <owl:Class rdf:about="http://www.ontology-of-units-of-measure.org/resource/om-2/Unit"/>
    


    <!-- http://www.w3.org/2006/time#Instant -->


    <owl:Class rdf:about="http://www.w3.org/2006/time#Instant"/>
    


    <!-- http://www.w3.org/2006/time#TemporalEntity -->


    <owl:Class rdf:about="http://www.w3.org/2006/time#TemporalEntity"/>
    


    <!-- https://github.com/TheWorldAvatar/ontoclimateadapt#AdaptationMeasure -->


    <owl:Class rdf:about="https://github.com/TheWorldAvatar/ontoclimateadapt#AdaptationMeasure">
        <rdfs:comment>A deliberate action, strategy, or intervention implemented to reduce the adverse impacts of climate change</rdfs:comment>
        <rdfs:isDefinedBy rdf:resource="https://github.com/TheWorldAvatar/ontoclimateadapt"/>
        <rdfs:label>AdaptationMeasure</rdfs:label>
    </owl:Class>
    


    <!-- https://github.com/TheWorldAvatar/ontoclimateadapt#AgeGroup -->


    <owl:Class rdf:about="https://github.com/TheWorldAvatar/ontoclimateadapt#AgeGroup">
        <rdfs:comment>A group of people whose ages fall within a specified range.</rdfs:comment>
        <rdfs:isDefinedBy rdf:resource="https://github.com/TheWorldAvatar/ontoclimateadapt"/>
        <rdfs:label>AgeGroup</rdfs:label>
    </owl:Class>
    


    <!-- https://github.com/TheWorldAvatar/ontoclimateadapt#AgeSpecificPopulationDensity -->


    <owl:Class rdf:about="https://github.com/TheWorldAvatar/ontoclimateadapt#AgeSpecificPopulationDensity">
        <rdfs:subClassOf rdf:resource="https://github.com/TheWorldAvatar/ontoclimateadapt#PopulationDensity"/>
        <rdfs:isDefinedBy rdf:resource="https://github.com/TheWorldAvatar/ontoclimateadapt"/>
        <rdfs:label>AgeSpecificPopulationDensity</rdfs:label>
    </owl:Class>
    


    <!-- https://github.com/TheWorldAvatar/ontoclimateadapt#AnnualFrequency -->


    <owl:Class rdf:about="https://github.com/TheWorldAvatar/ontoclimateadapt#AnnualFrequency">
        <rdfs:subClassOf rdf:resource="https://github.com/TheWorldAvatar/ontoclimateadapt#TemporalFrequency"/>
        <rdfs:comment>A temporal frequency representing the count of occurrences within a calendar year.</rdfs:comment>
        <rdfs:isDefinedBy rdf:resource="https://github.com/TheWorldAvatar/ontoclimateadapt"/>
        <rdfs:label>AnnualFrequency</rdfs:label>
    </owl:Class>
    


    <!-- https://github.com/TheWorldAvatar/ontoclimateadapt#AtmosphericScience -->


    <owl:Class rdf:about="https://github.com/TheWorldAvatar/ontoclimateadapt#AtmosphericScience"/>
    


    <!-- https://github.com/TheWorldAvatar/ontoclimateadapt#ClimateAdaptationAction -->


    <owl:Class rdf:about="https://github.com/TheWorldAvatar/ontoclimateadapt#ClimateAdaptationAction">
        <rdfs:subClassOf rdf:resource="https://github.com/TheWorldAvatar/ontoclimateadapt#AdaptationMeasure"/>
        <rdfs:comment>A concrete activity or measure undertaken to reduce the impacts of climate change or increase the resilience of human or natural systems.</rdfs:comment>
        <rdfs:isDefinedBy rdf:resource="https://github.com/TheWorldAvatar/ontoclimateadapt"/>
        <rdfs:label>ClimateAdaptationAction </rdfs:label>
    </owl:Class>
    


    <!-- https://github.com/TheWorldAvatar/ontoclimateadapt#ClimateChange -->


    <owl:Class rdf:about="https://github.com/TheWorldAvatar/ontoclimateadapt#ClimateChange">
        <rdfs:subClassOf rdf:resource="https://github.com/TheWorldAvatar/ontoclimateadapt#EarthSystemPhenomenon"/>
        <rdfs:subClassOf rdf:resource="https://github.com/TheWorldAvatar/ontoclimateadapt#EnvironmentalPhenomenon"/>
        <rdfs:comment>An Environmental Phenomenon that represents a persistent alteration in the statistical properties of the climate system.</rdfs:comment>
    </owl:Class>
    


    <!-- https://github.com/TheWorldAvatar/ontoclimateadapt#ClimateModel -->


    <owl:Class rdf:about="https://github.com/TheWorldAvatar/ontoclimateadapt#ClimateModel">
        <rdfs:comment>A computational model that applies mathematical equations to simulate the behaviour of the Earth’s climate system.</rdfs:comment>
        <rdfs:isDefinedBy rdf:resource="https://github.com/TheWorldAvatar/ontoclimateadapt"/>
        <rdfs:label>ClimateModel</rdfs:label>
    </owl:Class>
    


    <!-- https://github.com/TheWorldAvatar/ontoclimateadapt#EarthSystemPhenomenon -->


    <owl:Class rdf:about="https://github.com/TheWorldAvatar/ontoclimateadapt#EarthSystemPhenomenon">
        <rdfs:comment>A large-scale physical, chemical, or biological process that occurs within or across components of the Earth system.</rdfs:comment>
        <rdfs:isDefinedBy rdf:resource="https://github.com/TheWorldAvatar/ontoclimateadapt"/>
        <rdfs:label>EarthSystemPhenomenon</rdfs:label>
    </owl:Class>
    


    <!-- https://github.com/TheWorldAvatar/ontoclimateadapt#Ecology -->


    <owl:Class rdf:about="https://github.com/TheWorldAvatar/ontoclimateadapt#Ecology"/>
    


    <!-- https://github.com/TheWorldAvatar/ontoclimateadapt#Economy -->


    <owl:Class rdf:about="https://github.com/TheWorldAvatar/ontoclimateadapt#Economy"/>
    


    <!-- https://github.com/TheWorldAvatar/ontoclimateadapt#EnvironmentalPhenomenon -->


    <owl:Class rdf:about="https://github.com/TheWorldAvatar/ontoclimateadapt#EnvironmentalPhenomenon">
        <rdfs:comment>A naturally occurring process within the environment arising from interactions among biological, physical, or chemical components.</rdfs:comment>
        <rdfs:isDefinedBy rdf:resource="https://github.com/TheWorldAvatar/ontoclimateadapt"/>
        <rdfs:label>EnvironmentalPhenomenon</rdfs:label>
    </owl:Class>
    


    <!-- https://github.com/TheWorldAvatar/ontoclimateadapt#EnvironmentalScience -->


    <owl:Class rdf:about="https://github.com/TheWorldAvatar/ontoclimateadapt#EnvironmentalScience"/>
    


    <!-- https://github.com/TheWorldAvatar/ontoclimateadapt#GreenhouseGasEmission -->


    <owl:Class rdf:about="https://github.com/TheWorldAvatar/ontoclimateadapt#GreenhouseGasEmission"/>
    


    <!-- https://github.com/TheWorldAvatar/ontoclimateadapt#Heatwave -->


    <owl:Class rdf:about="https://github.com/TheWorldAvatar/ontoclimateadapt#Heatwave">
        <rdfs:subClassOf rdf:resource="https://github.com/TheWorldAvatar/ontoclimateadapt#MeteorologicalExtremeEvent"/>
        <rdfs:comment>A meteorological extreme event consisting of several consecutive days of unusually high temperatures relative to local climate norms.</rdfs:comment>
        <rdfs:isDefinedBy rdf:resource="https://github.com/TheWorldAvatar/ontoclimateadapt"/>
        <rdfs:label>Heatwave</rdfs:label>
    </owl:Class>
    


    <!-- https://github.com/TheWorldAvatar/ontoclimateadapt#HumanHealth -->


    <owl:Class rdf:about="https://github.com/TheWorldAvatar/ontoclimateadapt#HumanHealth"/>
    


    <!-- https://github.com/TheWorldAvatar/ontoclimateadapt#InfrastructureResilienceMeasure -->


    <owl:Class rdf:about="https://github.com/TheWorldAvatar/ontoclimateadapt#InfrastructureResilienceMeasure">
        <rdfs:subClassOf rdf:resource="https://github.com/TheWorldAvatar/ontoclimateadapt#AdaptationMeasure"/>
        <rdfs:comment>An adaptation measure that strengthens, upgrades, or redesigns physical infrastructure to withstand climate-related hazards.</rdfs:comment>
        <rdfs:isDefinedBy rdf:resource="https://github.com/TheWorldAvatar/ontoclimateadapt"/>
        <rdfs:label>InfrastructureResilienceMeasure </rdfs:label>
    </owl:Class>
    


    <!-- https://github.com/TheWorldAvatar/ontoclimateadapt#Location -->


    <owl:Class rdf:about="https://github.com/TheWorldAvatar/ontoclimateadapt#Location"/>
    


    <!-- https://github.com/TheWorldAvatar/ontoclimateadapt#MeteorologicalExtremeEvent -->


    <owl:Class rdf:about="https://github.com/TheWorldAvatar/ontoclimateadapt#MeteorologicalExtremeEvent">
        <rdfs:comment>Any atmospheric or weather-related phenomenon that deviates drastically from normal conditions and poses risks to humans, ecosystems, or infrastructure.</rdfs:comment>
        <rdfs:isDefinedBy rdf:resource="https://github.com/TheWorldAvatar/ontoclimateadapt"/>
        <rdfs:label>MeteorologicalExtremeEvent</rdfs:label>
    </owl:Class>
    


    <!-- https://github.com/TheWorldAvatar/ontoclimateadapt#MeteorologicalStation -->


    <owl:Class rdf:about="https://github.com/TheWorldAvatar/ontoclimateadapt#MeteorologicalStation">
        <rdfs:comment>A ground-based facility that measures atmospheric and weather variables such as temperature, humidity, precipitation, and wind.</rdfs:comment>
        <rdfs:isDefinedBy rdf:resource="https://github.com/TheWorldAvatar/ontoclimateadapt"/>
        <rdfs:label>MeteorologicalStation</rdfs:label>
    </owl:Class>
    


    <!-- https://github.com/TheWorldAvatar/ontoclimateadapt#MonthlyFrequency -->


    <owl:Class rdf:about="https://github.com/TheWorldAvatar/ontoclimateadapt#MonthlyFrequency">
        <rdfs:subClassOf rdf:resource="https://github.com/TheWorldAvatar/ontoclimateadapt#TemporalFrequency"/>
        <rdfs:comment>A temporal frequency representing the count of occurrences within a calendar month.</rdfs:comment>
        <rdfs:isDefinedBy rdf:resource="https://github.com/TheWorldAvatar/ontoclimateadapt"/>
        <rdfs:label>MonthlyFrequency</rdfs:label>
    </owl:Class>
    


    <!-- https://github.com/TheWorldAvatar/ontoclimateadapt#NumberOfHeatwaveDays -->


    <owl:Class rdf:about="https://github.com/TheWorldAvatar/ontoclimateadapt#NumberOfHeatwaveDays">
        <rdfs:subClassOf rdf:resource="http://www.ontology-of-units-of-measure.org/resource/om-2/Quantity"/>
        <rdfs:comment>A quantitative observation describing the total count of days during which heatwave conditions occur at a given location within a defined time interval.</rdfs:comment>
        <rdfs:isDefinedBy rdf:resource="https://github.com/TheWorldAvatar/ontoclimateadapt"/>
        <rdfs:label>NumberOfHeatwaveDays</rdfs:label>
    </owl:Class>
    


    <!-- https://github.com/TheWorldAvatar/ontoclimateadapt#OceanAcidification -->


    <owl:Class rdf:about="https://github.com/TheWorldAvatar/ontoclimateadapt#OceanAcidification"/>
    


    <!-- https://github.com/TheWorldAvatar/ontoclimateadapt#Paleoclimatology -->


    <owl:Class rdf:about="https://github.com/TheWorldAvatar/ontoclimateadapt#Paleoclimatology"/>
    


    <!-- https://github.com/TheWorldAvatar/ontoclimateadapt#PolicyIntervention -->


    <owl:Class rdf:about="https://github.com/TheWorldAvatar/ontoclimateadapt#PolicyIntervention">
        <rdfs:subClassOf rdf:resource="https://github.com/TheWorldAvatar/ontoclimateadapt#AdaptationMeasure"/>
        <rdfs:comment>A governance-led adaptation measure implemented through regulations, policies, legislation, incentives, or planning frameworks.</rdfs:comment>
        <rdfs:isDefinedBy rdf:resource="https://github.com/TheWorldAvatar/ontoclimateadapt"/>
        <rdfs:label>PolicyIntervention</rdfs:label>
    </owl:Class>
    


    <!-- https://github.com/TheWorldAvatar/ontoclimateadapt#PopulationDensity -->


    <owl:Class rdf:about="https://github.com/TheWorldAvatar/ontoclimateadapt#PopulationDensity">
        <rdfs:comment>A quantitative demographic indicator representing the number of individuals residing within a defined unit area of a geographic location.</rdfs:comment>
        <rdfs:isDefinedBy rdf:resource="https://github.com/TheWorldAvatar/ontoclimateadapt"/>
        <rdfs:label>PopulationDensity</rdfs:label>
    </owl:Class>
    


    <!-- https://github.com/TheWorldAvatar/ontoclimateadapt#SatelliteObservation -->


    <owl:Class rdf:about="https://github.com/TheWorldAvatar/ontoclimateadapt#SatelliteObservation">
        <rdfs:comment>A remote sensing measurement capturing key environmental or atmospheric variables of the Earth’s surface and climate system.</rdfs:comment>
        <rdfs:isDefinedBy rdf:resource="https://github.com/TheWorldAvatar/ontoclimateadapt"/>
        <rdfs:label>SatelliteObservation</rdfs:label>
    </owl:Class>
    


    <!-- https://github.com/TheWorldAvatar/ontoclimateadapt#SeaLevelRise -->


    <owl:Class rdf:about="https://github.com/TheWorldAvatar/ontoclimateadapt#SeaLevelRise"/>
    


    <!-- https://github.com/TheWorldAvatar/ontoclimateadapt#TemporalFrequency -->


    <owl:Class rdf:about="https://github.com/TheWorldAvatar/ontoclimateadapt#TemporalFrequency">
        <rdfs:comment>The regularity or recurrence pattern according to which an observation or aggregated value is defined, such as annually, monthly, or weekly.</rdfs:comment>
        <rdfs:isDefinedBy rdf:resource="https://github.com/TheWorldAvatar/ontoclimateadapt"/>
        <rdfs:label>TemporalFrequency</rdfs:label>
    </owl:Class>
    


    <!-- https://github.com/TheWorldAvatar/ontoclimateadapt#WeeklyFrequency -->


    <owl:Class rdf:about="https://github.com/TheWorldAvatar/ontoclimateadapt#WeeklyFrequency">
        <rdfs:subClassOf rdf:resource="https://github.com/TheWorldAvatar/ontoclimateadapt#TemporalFrequency"/>
        <rdfs:comment>A temporal frequency representing the count of occurrences within a calendar week.</rdfs:comment>
        <rdfs:isDefinedBy rdf:resource="https://github.com/TheWorldAvatar/ontoclimateadapt"/>
        <rdfs:label>WeeklyFrequency</rdfs:label>
    </owl:Class>
</rdf:RDF>



<!-- Generated by the OWL API (version 5.5.0.2023-01-14T12:41:38Z) https://github.com/owlcs/owlapi/ -->


